examples/preorders/InitFreezeRef.fst
@@ -1,0 +1,138 @@
+module InitFreezeRef
+
+open FStar.Preorder
+open FStar.Heap
+open FStar.ST
+
+private type rstate (a:Type) =
+  | Empty  : rstate a
+  | Mutable: v:a -> rstate a
+  | Frozen : v:a -> rstate a
+
+private let evolve_broken0 (a:Type) :relation (rstate a) =
+  fun r1 r2 ->
+  match r1, r2 with
+  | Empty,      Mutable _
+  | Mutable _,  Mutable _ -> True
+  | Mutable v1, Frozen v2 -> v1 == v2
+  | _, _ -> False
+
+(* private let evolve_broken (a:Type) :preorder (rstate a) = evolve_broken0 a
+   -- fails as it should *)
+
+private let evolve0 (a:Type) :relation (rstate a) =
+  fun r1 r2 ->
+  match r1, r2 with
+  | Empty,     _
+  | Mutable _, Mutable _
+  | Mutable _, Frozen _  -> True 
+  | Frozen v1, Frozen v2 -> v1 == v2
+  | _, _ -> False
+
+private let evolve (a:Type) :preorder (rstate a) = evolve0 a
+
+abstract type eref (a:Type) :Type0 = mref (rstate a) (evolve a)
+
+abstract let addr_of (#a:Type0) (r:eref a) :GTot nat = addr_of r
+
+private let readable_pred (#a:Type0) (r:eref a) :heap_predicate
+  = fun h -> h `contains` r /\ (~ (Empty? (sel h r)))
+
+abstract let readable (#a:Type0) (r:eref a) :Type0
+  = witnessed (readable_pred r)
+
+private let writable_pred (#a:Type0) (r:eref a) :heap_predicate
+  = fun h -> h `contains` r /\ (let x = sel h r in Empty? x \/ Mutable? x)
+
+(* abstract let writable (#a:Type0) (r:eref a) :Type0 = witnessed (writable_pred r)
+   -- fails as it should, why? *)
+
+abstract let writable_in (#a:Type0) (r:eref a) (h:heap) :Type0
+  = h `contains` r /\ (let x = sel h r in Empty? x \/ Mutable? x)
+
+private let frozen_at_pred (#a:Type0) (r:eref a) (x:a) :heap_predicate
+  = fun h -> h `contains` r /\ sel h r == Frozen x
+
+abstract let frozen_at (#a:Type0) (r:eref a) (x:a) :Type0
+  = witnessed (frozen_at_pred r x)
+
+abstract let sel (#a:Type0) (h:heap) (r:eref a) :GTot (option a)
+  = let x = sel h r in
+    match x with
+    | Empty     -> None
+    | Mutable x
+    | Frozen  x -> Some x
+
+abstract let alloc (a:Type0)
+  :ST (eref a) (requires (fun _       -> True))
+               (ensures  (fun h0 r h1 -> modifies !{} h0 h1 /\ r `writable_in` h1 /\ sel h1 r == None))
+  = ST.alloc #(rstate a) #(evolve a) Empty
+
+abstract let read (#a:Type0) (r:eref a{readable r})
+  :ST a (requires (fun _       -> True))
+        (ensures  (fun h0 x h1 -> h0 == h1 /\ sel h1 r == Some x))
+  = ST.gst_recall (readable_pred r);
+    let x = ST.read r in
+    match x with
+    | Mutable x
+    | Frozen  x -> x
+
+abstract let write (#a:Type0) (r:eref a) (x:a)
+  :ST unit (fun h0      -> r `writable_in` h0)
+           (fun h0 _ h1 -> modifies (Set.singleton (addr_of r)) h0 h1 /\
+	                readable r                                 /\
+	                r `writable_in` h1                         /\
+			sel h1 r == Some x)
+  = ST.write r (Mutable x);
+    gst_witness (readable_pred r)
+
+abstract let freeze (#a:Type0) (r:eref a{readable r})
+  :ST a (fun _       -> True)
+        (fun h0 x h1 -> modifies (Set.singleton (addr_of r)) h0 h1 /\
+	             sel h0 r == sel h1 r                       /\
+		     sel h0 r == Some x                         /\
+	             r `frozen_at` x)
+  = ST.recall r;
+    ST.gst_recall (readable_pred r);
+    let x = ST.read r in
+    let v, y =
+      match x with
+      | Mutable x
+      | Frozen  x -> x, Frozen x
+    in
+    ST.write r y;
+    gst_witness (frozen_at_pred r v);
+    v
+
+abstract let recall_freeze (#a:Type0) (r:eref a) (x:a{r `frozen_at` x})
+  :ST unit (requires (fun _       -> True))
+           (ensures  (fun h0 _ h1 -> h0 == h1 /\ sel h1 r == Some x))
+  = gst_recall (frozen_at_pred r x)
+
+// let alloc (a:Type) = alloc #_ #(evolve a) Empty
+// let read (#a:Type) (r:eref a) = match (!r) with | Mutable v | Frozen v -> v
+// private let write (#a:Type) (r:eref a) (v:a) = r := Mutable v
+// private let freeze (#a:Type) (r:eref a) = r := Frozen (Mutable?.v !r)
+// (* TODO: for some reason needed to mark these as private, otherwise
+// ./InitFreezeMST.fst(35,41-35,43): (Error) Interface of InitFreezeMST violates its abstraction (add a 'private' qualifier to 'write'?): Too many arguments to function of type a:Type0 -> Prims.Tot (Preorder.preorder (InitFreezeMST.rstate a)); got 3 arguments (see also ./STx.fst(95,25-95,34)) *)
+
+// assume val complex_procedure (r:eref int) : St unit
+
+// let main() : St unit =
+//   let r = alloc int in
+//   (* ignore (read r) -- fails like it should *)
+//   write r 42;
+//   ignore (read r);
+//   write r 0;
+//   witness_token r (fun rs -> ~(Empty? rs));
+//   freeze r;
+//   (* write r 7; -- fails like it should *)
+//   ignore (read r);
+//   witness_token r (fun rs -> rs == Frozen 0);
+//   complex_procedure r;
+//   (* ignore (read r); -- fails like it should *)
+//   recall_token r (fun rs -> ~(Empty? rs));
+//   let x = read r in
+//   (* assert (x == 0) -- fails like it should *)
+//   recall_token r (fun rs -> rs == Frozen 0);
+//   assert (x == 0)
