examples/preorders/InitFreezeRefClient.fst
@@ -1,0 +1,30 @@
+module InitFreezeRefClient
+
+open FStar.Heap
+open FStar.ST
+open InitFreezeRef
+
+assume val complex_routine: unit -> ST unit (fun _ -> True) (fun _ _ _ -> True)
+
+let test () :ST unit (requires (fun _ -> True)) (ensures (fun _ _ _ -> True)) =
+  let r = alloc int in
+  //let x = read r in  -- can't read, rightfully so
+  write r 0;
+  let x = read r in
+  assert (x = 0);
+
+  write r 1;
+  let x = read r in
+  assert (x = 1);
+
+  let x = freeze r in
+
+  //write r 2  -- fails, rightfully so
+
+  complex_routine ();
+
+  recall_freeze r x;
+
+  let y = read r in
+  assert (x = y);
+  ()
